theories/program_logic/weakestpre.v
@@ -306,23 +306,23 @@ Section proofmode_classes.
 
   Global Instance elim_acc_wp {X} E1 E2 α β γ e s Φ :
     Atomic (stuckness_to_atomicity s) e →
-    ElimAcc (X:=X) (fupd E1 E2) (fupd E2 E1)
+    ElimAcc (X:=X) True (fupd E1 E2) (fupd E2 E1)
             α β γ (WP e @ s; E1 {{ Φ }})
             (λ x, WP e @ s; E2 {{ v, |={E2}=> β x ∗ (γ x -∗? Φ v) }})%I.
   Proof.
-    intros ?. rewrite /ElimAcc.
+    intros ? _.
     iIntros "Hinner >Hacc". iDestruct "Hacc" as (x) "[Hα Hclose]".
     iApply (wp_wand with "(Hinner Hα)").
     iIntros (v) ">[Hβ HΦ]". iApply "HΦ". by iApply "Hclose".
   Qed.
 
   Global Instance elim_acc_wp_nonatomic {X} E α β γ e s Φ :
-    ElimAcc (X:=X) (fupd E E) (fupd E E)
+    ElimAcc (X:=X) True (fupd E E) (fupd E E)
             α β γ (WP e @ s; E {{ Φ }})
             (λ x, WP e @ s; E {{ v, |={E}=> β x ∗ (γ x -∗? Φ v) }})%I.
   Proof.
     rewrite /ElimAcc.
-    iIntros "Hinner >Hacc". iDestruct "Hacc" as (x) "[Hα Hclose]".
+    iIntros (_) "Hinner >Hacc". iDestruct "Hacc" as (x) "[Hα Hclose]".
     iApply wp_fupd.
     iApply (wp_wand with "(Hinner Hα)").
     iIntros (v) ">[Hβ HΦ]". iApply "HΦ". by iApply "Hclose".
